vipersemabstract/AbstractSemantics.thy
@@ -475,6 +475,19 @@ proof
     by (metis (mono_tags, lifting) assms(1) max_projection_prop_def max_projection_prop_stable_stabilize wf_expE)
 qed
 
+definition atrue where
+  "atrue \<Delta> = {\<omega>. typed \<Delta> \<omega>}"
+
+lemma fvaA_atrue_empty[simp]:
+  "free_vars \<Delta> (atrue \<Delta>) = {}"
+  sorry (* fvA \<Delta> *)
+
+lemma free_vars_agree:
+  assumes "typed_store \<Delta> \<sigma>1"
+      and "typed_store \<Delta> \<sigma>2"
+      and "equal_on_set (free_vars \<Delta> A) \<sigma>1 \<sigma>2"
+    shows "((Ag \<sigma>1, \<gamma>) \<in> A \<longleftrightarrow> (Ag \<sigma>2, \<gamma>) \<in> A)"
+  sorry (* TODO: free_vars *)
 
 end
 
